OpenSea.v
@@ -1,0 +1,215 @@
+Require Import FullSpecificationSmartContracts.Common.
+
+Local Open Scope bool_scope.
+
+Definition InitInput : Set :=
+  unit.
+
+(** The init outputs a new token kind *)
+Definition InitOutput : Set :=
+  TokenKind.
+
+Module State.
+  Definition t : Set :=
+    unit.
+End State.
+
+(** Entrypoints of the contract *)
+Module Command.
+  Inductive t {payment_token_kind : InitOutput} : Set -> Set :=
+  | FulfillOrder
+      (nft_type : TokenKind)
+      (nft_quantity : TokenQuantity nft_type)
+      (amount : TokenQuantity payment_token_kind) :
+      t bool
+  .
+  Arguments t : clear implicits.
+End Command.
+
+Definition smart_contract :
+  SmartContract.t
+    InitInput
+    InitOutput
+    Command.t
+    State.t :=
+{|
+  SmartContract.init _sender _input :=
+    let! payment_token_kind := M.MakeAction Action.CreateTokenKind in
+    M.Pure (Some (payment_token_kind, tt));
+  SmartContract.call A payment_token_kind sender command state :=
+    match command in Command.t _ A return M.t (option (A * _)) with
+    | Command.FulfillOrder nft_type nft_quantity amount =>
+      let! user := M.MakeAction (Action.FindUserWithEnoughBalance nft_type nft_quantity) in
+      match user with
+      | Some user =>
+        let! selling_price :=
+          M.MakeAction (Action.SellingPriceForNft payment_token_kind nft_type user) in
+        match selling_price with
+        | Some selling_price =>
+          let! is_payment_success :=
+            M.MakeAction (Action.Transfer payment_token_kind sender user selling_price) in
+          let! is_nft_transfer_success :=
+            M.MakeAction (Action.Transfer nft_type user sender nft_quantity) in
+          M.Pure (Some (is_payment_success && is_nft_transfer_success, state))
+        | None =>
+          M.Pure (Some (false, state))
+        end
+      | None =>
+        M.Pure (Some (false, state))
+      end
+    end
+|}.
+
+Module IsSafe.
+  Lemma is_safe : NoStealing.InSmartContract.t smart_contract.
+  Proof.
+    constructor; intros; cbn.
+    { (* init *)
+      unfold NoStealing.InRun.t; cbn.
+      destruct Primitives.create_token_kind.
+      apply ActionTree.Forall.Let. {
+        apply ActionTree.Forall.MakeAction.
+        cbn.
+        trivial.
+      }
+      apply ActionTree.Forall.Pure.
+    }
+    { (* call *)
+      destruct command.
+      { (* FulfillOrder *)
+        unfold NoStealing.InRun.t; cbn.
+        destruct Primitives.find_user_with_enough_balance; cbn.
+        { (* We found a user with enough balance *)
+          destruct Primitives.selling_price_for_nft; cbn.
+          { (* We found a selling price *)
+            destruct Primitives.transfer; cbn.
+            { (* The payment transfer succeeded *)
+              destruct Primitives.transfer; cbn.
+              { (* The NFT transfer succeeded *)
+                apply ActionTree.Forall.Let. {
+                  apply ActionTree.Forall.MakeAction.
+                  cbn.
+                  trivial.
+                }
+                apply ActionTree.Forall.Let. {
+                  apply ActionTree.Forall.MakeAction.
+                  cbn.
+                  trivial.
+                }
+                apply ActionTree.Forall.Let. {
+                  apply ActionTree.Forall.MakeAction.
+                  cbn.
+                  trivial.
+                }
+                apply ActionTree.Forall.Let. {
+                  apply ActionTree.Forall.MakeAction.
+                  cbn.
+                  (* TODO: make another formalization so that we can explicit that we are actually
+                     not stealing the NFTs, as we just made the payment before. *)
+                  admit.
+                }
+                apply ActionTree.Forall.Pure.
+              }
+              { (* The NFT transfer failed *)
+                apply ActionTree.Forall.Let. {
+                  apply ActionTree.Forall.MakeAction.
+                  cbn.
+                  trivial.
+                }
+                apply ActionTree.Forall.Let. {
+                  apply ActionTree.Forall.MakeAction.
+                  cbn.
+                  trivial.
+                }
+                apply ActionTree.Forall.Let. {
+                  apply ActionTree.Forall.MakeAction.
+                  cbn.
+                  trivial.
+                }
+                apply ActionTree.Forall.Let. {
+                  apply ActionTree.Forall.MakeAction.
+                  cbn.
+                  (* Same issue as above *)
+                  admit.
+                }
+                apply ActionTree.Forall.Pure.
+              }
+            }
+            { (* The payment transfer failed *)
+              destruct Primitives.transfer; cbn.
+              { (* The NFT transfer succeeded *)
+                apply ActionTree.Forall.Let. {
+                  apply ActionTree.Forall.MakeAction.
+                  cbn.
+                  trivial.
+                }
+                apply ActionTree.Forall.Let. {
+                  apply ActionTree.Forall.MakeAction.
+                  cbn.
+                  trivial.
+                }
+                apply ActionTree.Forall.Let. {
+                  apply ActionTree.Forall.MakeAction.
+                  cbn.
+                  trivial.
+                }
+                apply ActionTree.Forall.Let. {
+                  apply ActionTree.Forall.MakeAction.
+                  cbn.
+                  (* Same issue as above *)
+                  admit.
+                }
+                apply ActionTree.Forall.Pure.
+              }
+              { (* The NFT transfer failed *)
+                apply ActionTree.Forall.Let. {
+                  apply ActionTree.Forall.MakeAction.
+                  cbn.
+                  trivial.
+                }
+                apply ActionTree.Forall.Let. {
+                  apply ActionTree.Forall.MakeAction.
+                  cbn.
+                  trivial.
+                }
+                apply ActionTree.Forall.Let. {
+                  apply ActionTree.Forall.MakeAction.
+                  cbn.
+                  trivial.
+                }
+                apply ActionTree.Forall.Let. {
+                  apply ActionTree.Forall.MakeAction.
+                  cbn.
+                  (* Same issue as above *)
+                  admit.
+                }
+                apply ActionTree.Forall.Pure.
+              }
+            }
+          }
+          { (* We did not find a user with enough balance *)
+            apply ActionTree.Forall.Let. {
+              apply ActionTree.Forall.MakeAction.
+              cbn.
+              trivial.
+            }
+            apply ActionTree.Forall.Let. {
+              apply ActionTree.Forall.MakeAction.
+              cbn.
+              trivial.
+            }
+            apply ActionTree.Forall.Pure.
+          }
+        }
+        { (* We did not find a user with enough balance *)
+          apply ActionTree.Forall.Let. {
+            apply ActionTree.Forall.MakeAction.
+            cbn.
+            trivial.
+          }
+          apply ActionTree.Forall.Pure.
+        }
+      }
+    }
+  Admitted.
+End IsSafe.
